# Additional Exercise 6
Show that $$a_{n} = 3  \cdot 2^{n} + 7 \cdot 5^{n}$$ is a solution to the recurrence relation $$a_{n} = 7a_{n-1} - 10a_{n-2}$$. 
What would the initial conditions need to be for this to be the closed formula for the sequence?

You can start by finding some of the terms using the closed formula:

$$a_{0} = 3  \cdot 2^{0} + 7 \cdot 5^{0} = 10$$

$$a_1 = 3 \cdot 2^1 + 7 \cdot 5^1 = 41$$

$$a_2 = 3 \cdot 2^2 + 7 \cdot 5^2 = 187$$

$$a_3 = 3 \cdot 2^3 + 7 \cdot 5^3 = 899$$

$$a_4 = 3 \cdot 2^4 + 7 \cdot 5^4 = 4423$$

$$a_5 = 3 \cdot 2^5 + 7 \cdot 5^5 = 21971$$

$$a_6 = 3 \cdot 2^6 + 7 \cdot 5^6 = 109567$$


Then, you can check to see if they fit the recurrence relation

According to the relation: $$a_2 = 7a_1 - 10a_0 = 7 \cdot 41 - 10 \cdot 10 = 187$$, which matches the $$a_2$$ term from the closed formula

When calculating the rest of the terms, you get

$$a_2 = 7a_1 - 10a_0 = 187$$

$$a_3 = 7a_2 - 10a_1 = 899$$

$$a_4 = 7a_3 - 10a_2 = 4423$$

$$a_5 = 7a_4 - 10a_3 = 21971$$

$$a_6 = 7a_5 - 10a_4 = 109567$$

All of the terms from the reccurence relation match the terms from the closed formula, showing that $$a_{n} = 3  \cdot 2^{n} + 7 \cdot 5^{n}$$ is a solution to $$a_{n} = 7a_{n-1} - 10a_{n-2}$$

However, the initial conditions of $$a_0 = 10$$ and $$a_1 = 41$$ must be met for the formulas to match
